LogRel/LemmasLR.v
@@ -1,0 +1,88 @@
+Require Import LogRel.LR.
+Require Import Stlc.SpecSyntax.
+Require Import Stlc.SpecEvaluation.
+Require Import Stlc.LemmasEvaluation.
+Require Import Stlc.SpecTyping.
+Require Import Utlc.SpecSyntax.
+Require Import Utlc.SpecEvaluation.
+Require Import Utlc.LemmasEvaluation.
+Require Import Utlc.Inst.
+
+Require Import Omega.
+Require Import Min.
+
+Module S.
+  Include Stlc.SpecSyntax.
+  Include Stlc.SpecEvaluation.
+  Include Stlc.LemmasEvaluation.
+End S.
+Module U.
+  Include Utlc.SpecSyntax.
+  Include Utlc.SpecEvaluation.
+  Include Utlc.LemmasEvaluation.
+End U.
+
+Section Obs.
+  Lemma obs_mono {d W' W ts tu} :
+    lev W' ≤ lev W →
+    Obs d W ts tu →
+    Obs d W' ts tu.
+  Proof.
+    intros fw obs.
+    destruct d; simpl in *; 
+    eauto using S.TerminatingN_lt, U.TerminatingN_lt.
+  Qed.
+  
+  Lemma obs_antired {ts ts' tu tu' W' W d i j} :
+    S.evaln ts ts' i →
+    U.evaln tu tu' j →
+    W' ≤ W →
+    lev W' + min i j ≥ lev W →
+    Obs d W' ts' tu' →
+    Obs d W ts tu.
+  Proof.
+    intros es eu fw sge obs.
+    destruct d; unfold Obs in *; intros ttsw.
+    - cut (tu'⇓).
+      + refine (U.termination_closed_under_antireductionStar _).
+        eauto using evaln_to_evalStar.
+      + apply obs; clear obs.
+        rewrite -> (S.TerminatingN_evaln (lev W') es).
+        refine (S.TerminatingN_lt ttsw _).
+        enough (min i j ≤ i) by omega.
+        auto using le_min_l.
+    - refine (S.termination_closed_under_antireductionStar _ _).
+      + refine (S.evaln_to_evalStar es).
+      + apply obs.
+        rewrite -> (U.TerminatingN_evaln (lev W') eu).
+        refine (U.TerminatingN_lt ttsw _).
+        enough (min i j ≤ j) by omega.
+        auto using le_min_r.
+  Qed.
+End Obs.
+
+Section ClosedLR.
+  Lemma contrel_mono {d W τ Cs Cu W'} :
+    W' ≤ W → contrel d W τ Cs Cu → contrel d W' τ Cs Cu.
+  Proof.
+    intros fw cr. simpl.
+    intros W'' fw' vs vu vr.
+    apply cr; try omega; auto.
+  Qed.
+  
+  Lemma termrel_antired (ts ts' : S.Tm) (tu tu' : U.UTm) (W' W : World) d τ i j :
+    S.evaln ts ts' i →
+    (forall C, ECtx C → U.evaln (U.pctx_app tu C) (U.pctx_app tu' C) j) →
+    W' ≤ W →
+    lev W' + min i j ≥ lev W →
+    termrel d W' τ ts' tu' →
+    termrel d W τ ts tu.
+  Proof.
+    intros es eu fw sge tr.
+    unfold termrel, termrel'.
+    intros Cs Cu ecs ecu cr.
+    refine (obs_antired _ _ fw sge _); eauto using S.evaln_ctx.
+    apply tr; auto. 
+    refine (contrel_mono fw cr).
+  Qed.
+End ClosedLR.
